doc/simple/coq/UtilityEnv.v
@@ -1,0 +1,64 @@
+Require Import DeclDef.
+Require Import AlgoDef.
+Require Import LibLN.
+
+Set Implicit Arguments.
+
+Lemma union_left :forall {A} (x:A) E F,
+    x \in E ->
+    x \in (E \u F).
+Proof.
+  intros* H.
+  assert(subset E (E \u F)). apply subset_union_weak_l.
+  apply* (H0 x).
+Qed.
+
+Lemma union_right :forall {A} (x:A) E F,
+    x \in E ->
+    x \in (F \u E).
+Proof.
+  intros* H.
+  assert(subset E (F \u E)). apply subset_union_weak_r.
+  apply* (H0 x).
+Qed.
+
+Lemma split_context : forall {A} (G:env A) x,
+    x \in (dom G) ->
+    exists G1 G2 v, G = G1 & (x ~ v) & G2.
+Proof.
+  intros* HX.
+  induction G using env_ind.
+  simpl_dom. rewrite in_empty in HX. inversion HX.
+  destruct (eq_var_dec x x0); subst.
+  exists* G (empty: env A) v. rewrite concat_empty_r. auto.
+  simpl_dom.
+  rewrite in_union in HX. destruct HX as [HX1 | HX2].
+  rewrite* in_singleton in HX1.
+  apply IHG in HX2. destruct HX2 as (G1 & G2 & v0 & HX); subst.
+  exists* G1 (G2 & x0 ~ v) v0. rewrite* concat_assoc.
+Qed.
+
+Lemma tail_exists_eq : forall {A} x vx y vy (E F G: env A),
+    x <> y ->
+    E & x ~ vx = F & y ~ vy & G ->
+    exists G1, G = G1 & x ~ vx.
+Proof.
+  introv Hxy H.
+  induction G using env_ind.
+  rewrite concat_empty_r in H. apply eq_push_inv in H.
+  destruct H as [H1  H2]. apply Hxy in H1. inversion H1.
+  rewrite concat_assoc in H.
+  apply eq_push_inv in H; subst.
+  destruct H as [xeq [veq Eeq]]; subst.
+  exists* G.
+Qed.
+
+Lemma ok_non_eq : forall {A} x vx y vy (E F G: env A),
+    ok (E & x ~ vx & F & y ~ vy & G) -> x <> y.
+Proof.
+  introv H.
+  apply ok_middle_inv in H. destruct H as [H _].
+  simpl_dom. apply notin_union in H.  destruct H as [H _].
+  apply notin_union in H.  destruct H as [_ H].
+  apply* notin_singleton.
+Qed.
